backup

Protocol/SAMLProtocol.fst
@@ -1,22 +1,20 @@
 module Protocol
 
-type prin = string
-type pubkey :: prin => *
-type privkey :: prin => *
-type dsig = string
-type resource = bytes
-type uri = string
-type nonce = string (*How to secure uniqueness? P-kind?*)
-type samlmessage = string
-type assertion = string
+open Network
 
-type message =
-  | HttpGet: uri -> message
-  | SamlProtocolMessage: prin -> samlmessage -> dsig -> message
-  | Credentials: string -> string -> nonce -> message
-  | ChallengeMessage: nonce -> message
-  | Resource: uri -> message
-  | Failed: int -> message
+type assertiontoken = string
+type id = string
+
+
+type Assertion =
+  | UnsignedAssertion: assertiontoken -> 
+
+type SamlMessage =
+  | Login: uri -> SamlMessage
+  | AuthnRequest: prin -> samlmessage -> dsig -> SamlMessage
+  | ResponseMessage: uri -> SamlMessage
+  | LoginResponse: int -> SamlMessage
+  | Failed: int -> SamlMessage
 
 type SamlStatus =
   | Success: SamlStatus
@@ -27,36 +25,7 @@ type SamlStatus =
 type Log :: prin => samlmessage => E
 type Log2 :: string => string => nonce => E
 
-(*Crypto functions*)
-val Keygen:  p:prin
-          -> (pubkey p * privkey p)
+val SendSaml: prin -> SamlMessage -> unit
+val RecieveSaml: prin -> SamlMessage 
 
-val Sign:  p:prin
-        -> privkey p
-        -> msg:samlmessage{Log p msg}
-        -> dsig
-
-val VerifySignature: p:prin
-        -> pubkey p 
-        -> msg:samlmessage
-        -> dsig
-        -> b:bool{b=true ==> Log p msg}
-
-val AuthenticateUser: user:string
-        -> password:string
-        -> challenge:nonce
-        -> b:bool{b=true ==> Log2 user password challenge}
-
-val Send: prin -> message -> unit
-val Recieve: prin -> message 
-
-(*Crypto functions*)
-extern reference Crypto {language="F#";
-            dll="Crypto";
-            namespace="";
-            classname="Crypto"}
-
-extern Crypto val KeyGenExt: p:prin
-          -> (pubkey p * privkey p)
-
-
+val IssuerAssertion: issuer:prin -> subject:prin -> audience:prin -> inresto:id -> assertiontoken
